inv te mplate

acl2/books/reduce-v2/reduce-v2.lisp
@@ -4,8 +4,6 @@
 (set-induction-depth-limit 1)
 
 
-
-
 ; PROOF PLAN
 ; 
 ; - step 1: show that erl-step of a wtree returns a wtree
@@ -41,8 +39,7 @@
     (wtree0-p (erl-step net) (erl-step net0) (omap::size (erl-step net))))
   :enable (wtree0-p erl-step proc-receive)))
 
-
-
+; TODO for Mark
 (defrule wtree-p-of-erl-step
   (implies
     (and (network-p net) (wtree-p net))
@@ -51,59 +48,460 @@
 
 ; TODO maybe I should make wtree-p a fixtype?
 ; Also, do I need to state that the wtree must have a root?
+; How will fuel work?
 
-; First TODO: maybe I should combine inbox new and inbox tried???
-; How will fuel work???
+; TODO: inbox-tried
+                ; messages valid, but does not contain ClHd.
+                ; forall received messages, sender has terminated. Thus, can use
+                ; the inv from above
+                ; 
+; same as blocked, but inbox-tried is empty.
+          ; inbox new messages are valid.
+          ; Message valid means
+          ;  - there exists x in CPids with message's pid
+          ;  - message contains reduce up
+          ;  - val in message is the val in terminated message.
 
+
+
+(define sum ((n natp))
+  (b* ((n (nfix n))
+       ((if (= n 0)) 0))
+      (+ n (sum (1- n)))))
+
+; (sum-range 0 2) -> 3
+; (sum-range 1 2) -> 3
+; (sum-range 1 3) -> 6
+; (sum-range 5 6) -> 11
+(define sum-range ((i natp) (j natp))
+  :returns (n natp)
+  :measure (acl2-count (- (nfix j) (nfix i)))
+  (b* ((i (nfix i))
+       (j (nfix j))
+       ((if (< j i)) 0)
+       ((if (equal i j)) i))
+      (+ i (sum-range (+ 1 i) j)))
+  ///
+    (defcong nat-equiv equal (sum-range i j) 1)
+    (defcong nat-equiv equal (sum-range i j) 2)
+    
+    (defrule sum-range-of-add
+      (implies
+        (and (natp i) (natp j) (natp n) (<= i j) (< j n))
+        (equal (+ (sum-range i j) (sum-range (+ j 1) n))
+               (sum-range i n))))
+    (defrule sum-range-of-sum
+      (implies
+        (and (natp i) (natp j) (<= i j))
+        (equal (sum-range i j) (- (sum j) (sum (1- i)))))
+      :enable sum)
+    (defrule sum-range-of-one
+      (implies (natp j) (equal (sum-range 1 j) (sum j)))
+      :enable sum)
+    (defrule sum-range-of-zero
+      (implies (natp j) (equal (sum-range 0 j) (sum j)))
+      :enable sum))
+
+; forall messages in inbox
+; the sender exists in cpids and net,
+; the sender is terminated,
+; the received message has the has value as the terminated
+; process' value.
+; TODO: Should I make sure there are no double messages?
+(define received-messages-wf
+  ((inbox erl-vlst-p) (cpids erl-vlst-p) (net network-p))
+  :returns (r booleanp)
+  :measure (acl2-count (erl-vlst-fix inbox))
+  (b* ((inbox (erl-vlst-fix inbox))
+       (cpids (erl-vlst-fix cpids))
+       (net (network-fix net))
+       ((unless inbox) t)
+       (m (car inbox))
+       ((unless (equal (erl-val-kind m) :tuple)) nil)
+       (lst (erl-val-tuple->lst m))
+       ; message should be in form: {sender, direction, value}
+       ((unless (equal (len lst) 3)) nil)
+       (sender (car lst))
+       (dir (cadr lst))
+       (val (caddr lst))
+       ; the sender exists
+       ((unless (member-equal sender cpids)) nil)
+       ((unless (omap::assoc sender net)) nil)
+       (sproc (omap::lookup sender net))
+       ; the sender must have terminated
+       ((unless (equal (proc->ps sproc) :terminated)) nil)
+       ; the sender must have sent its own value
+       ; which will be equal to its sum-range.
+       ; This is simply an implementation detail,
+       ; and the invariant should depend on a more general fact.
+       (sval (erl-state->in (proc->s sproc)))
+       ((unless (equal sval val)) nil)
+       ; The direction is up
+       ((unless
+          (and (equal (erl-val-kind dir) :atom)
+               (equal (erl-val-atom->val dir) 'reduce-up)))))
+      (received-messages-wf (cdr inbox) cpids net))
+  ///
+    (defcong erl-vlst-equiv equal (received-messages-wf x y z) 1)
+    (defcong erl-vlst-equiv equal (received-messages-wf x y z) 2)
+    (defcong network-equiv equal (received-messages-wf x y z) 3))
+
+; more helpers
+(define inbox-contains ((inbox erl-vlst-p) (pid pid-p))
+  :returns (r booleanp)
+  :measure (acl2-count (erl-vlst-fix inbox))
+  (b* ((inbox (erl-vlst-fix inbox))
+       (pid (pid-fix pid))
+       ((unless inbox) nil)
+       (m (car inbox))
+       ((if (equal m pid)) t))
+      (inbox-contains (cdr inbox) pid))
+  ///
+    (defcong erl-vlst-equiv equal (inbox-contains x y) 1)
+    (defcong pid-equiv equal (inbox-contains x y) 2))
+
+
+(defrule head-of-outbox
+  (implies
+    (and (not (omap::emptyp m)) (outbox-p m))
+    (and
+      (pid-p (mv-nth 0 (omap::head m)))
+      (erl-vlst-p (mv-nth 1 (omap::head m)))))
+  :enable outbox-p)
+
+(defrule head-of-outbox-consp
+  (implies
+    (and
+      (not (omap::emptyp m)) (outbox-p m)
+      (mv-nth 1 (omap::head m)))
+    (consp (mv-nth 1 (omap::head m))))
+  :enable (outbox-p erl-vlst-p)
+  :disable head-of-outbox
+  :use (:instance head-of-outbox))
+
+  ; if outbox not null
+  ;   it has a single message, same as the process's value
+  ; if the outbox is null
+  ; if the parent
+  ;   is terminated ok
+  ;   else
+  ;     either inbox-new or inbox-tried contains the message
+  ;     or Cpids does not contain the message,
+  ;     ??? index of Chd is greater than self's index
+(define sent-message-wf
+  ((self proc-p) (outbox outbox-p) (parent erl-val-p) (net network-p))
+  :returns (r booleanp)
+  :enabled t
+  ;guard-hints (("Goal" :use (:insrance )))
+  (b* ((self (proc-fix self))
+       (outbox (outbox-fix outbox))
+       (parent (erl-val-fix parent))
+       (net (network-fix net)) 
+       ; the root does not send messages
+       ((unless (pid-p parent)) (omap::emptyp outbox))
+       ; the parent exists, though we know this when
+       ;  calling this helper.
+       ((unless (omap::assoc parent net)) nil)
+       (pproc (omap::lookup parent net))
+       (ps (proc->ps pproc))
+       ; We can assume that self is terminated.
+       (val (erl-state->in (proc->s self))))
+      (if (omap::emptyp outbox)
+          (case ps
+            (:terminated t)
+            ; message must be in the correct inbox
+            ; the other helper already checks that it
+            ; is the correct message, so here I
+            ; only need to check that the message was
+            ; received. 
+            (:idle
+              (inbox-contains (proc->inbox-new pproc)
+                              (proc->pid self)))
+            (:blocked
+              ; same here, the main invariant makes
+              ; sure other properties are correct.
+              (or
+                (inbox-contains (proc->inbox-new pproc)
+                                (proc->pid self))
+                (inbox-contains (proc->inbox-tried pproc)
+                                (proc->pid self))))
+            (:receive
+              (inbox-contains (proc->inbox-new pproc)
+                              (proc->pid self))))
+          (b* ((ms (omap::head-val outbox))
+               ; there is a single message
+               ((unless (and ms (not (cdr ms)))) nil)
+               (m (car ms))
+               ; message is for the parent
+               ((unless (equal (omap::head-key outbox) parent)) nil)
+               ; this implementation sends no other message
+               ((unless (omap::emptyp (omap::tail outbox))) nil)
+               ; message should be in form: {sender, direction, value} 
+               ((unless (equal (erl-val-kind m) :tuple)) nil)
+               (lst (erl-val-tuple->lst m))
+               ((unless (equal (len lst) 3)) nil)
+               ((unless (equal (car lst) (proc->pid self))) nil)
+               ((unless (equal (cadr lst) 'reduce_up)) nil)
+               ((unless (equal (caddr lst) val)) nil))
+              t)))
+  ///
+    (defcong proc-equiv equal (sent-message-wf a b c d) 1)
+    (defcong outbox-equiv equal (sent-message-wf a b c d) 2)
+    (defcong erl-val-equiv equal (sent-message-wf a b c d) 3)
+    (defcong network-equiv equal (sent-message-wf a b c d) 4))
+
+(define reduce-receive-klst-p ((klst erl-klst-p) (rbind bind-p))
+  :returns (r booleanp)
+  :enabled t
+  (b* ((klst (erl-klst-fix klst))
+       (rbind (bind-fix rbind))
+       ((unless (equal (len klst) 3)) nil)
+       (k1 (car klst))
+       (k2 (cadr klst))
+       (k3 (caddr klst))
+       ; All continuations must have enough fuel, lets say 100
+       ((unless (> (erl-k->fuel k1) 100)) nil)
+       ((unless (> (erl-k->fuel k2) 100)) nil)
+       ((unless (> (erl-k->fuel k3) 100)) nil)
+       ; The three continuations must be the following:
+       (kont1 (erl-k->kont k1))
+       (kont2 (erl-k->kont k1))
+       (kont3 (erl-k->kont k1)))
+      (and
+        (equal
+          kont1
+          (make-kont-receive
+            :clauses '(((cases (:tuple (:cons (:var childhd)
+                                             (:cons (:var righttotal) (:nil)))))
+                        (guards)
+                        (body (:call sum_reduce
+                                     (:cons (:var parentpid)
+                                            (:cons (:var childtl)
+                                                   (:cons (:binop + (:var lefttotal)
+                                                                    (:var righttotal))
+                                                          (:nil))))))))))
+        (equal kont2 (make-kont-exprs :exprs nil))
+        (equal kont3
+          (make-kont-function-return
+            :bind rbind
+            :module 'local))))
+  ///
+    (defcong erl-klst-equiv equal (reduce-receive-klst-p klst rbind) 1)
+    (defcong bind-equiv equal (reduce-receive-klst-p klst rbind) 2))
+
+; TODO: now we need pid-list-p of children!
+; '???' notes constrains that might not be necessary.
 (define inv ((pid pid-p) (net network-p))
   :ignore-ok t
   :returns (r booleanp)
+  :guard-hints
+    (("Goal" :in-theory (enable omap::from-lists)))
   (b* ((pid (pid-fix pid))
        (net (network-fix net))
        ((unless (omap::assoc pid net)) nil)
        (proc (omap::lookup pid net))
-       ((unless (leaf-p proc)) t)
+       ((unless (or (leaf-p proc) (root-p proc))) t)
        (ps (proc->ps proc))
-       (bind (erl-state->bind (proc->s ps)))
+       (bind (erl-state->bind (proc->s proc)))
        (parent (omap::lookup 'Parent bind))
-       (children (omap::lookup 'Children bind))
-       (index (omap::lookup 'Index bind)))
+       (children (erl-val-cons->lst (omap::lookup 'ChildPids bind)))
+       (index (erl-val-integer->val (omap::lookup 'Index bind))))
       (case ps
         (:idle
-          ; equal proc (make-reduce-proc ...)
-          )
+          ; If the process has not been run yet, it is has not changed
+          ; at all since it was spawned. However, it might have received
+          ; messages.
+          (b* (; init-proc simulates a proc that has just been spawned,
+               ;  having received no messages.
+               (init-proc (make-reduce-proc pid parent children index))
+               ((unless (equal (proc->s proc) (proc->s init-proc))) nil)
+               ((unless (equal (proc->klst proc) (proc->klst init-proc))) nil)
+               ((unless (null (proc->inbox-tried proc))) nil)
+               (inbox (proc->inbox-new proc)))
+              (received-messages-wf inbox children net)))
         (:terminated
-          ; /\ equal s->in f(i, j) or i
-          ; /\ if leaf
-          ;    \/
-          ;     /\ outbox = empty
-          ;     /\ parent:
-          ;         \/ message in parent inbox
-          ;         \/ parent already received
-          ;   \/ message in outbox
-          ; /\ if root, empty outbox
-          ; /\ message contains f(i, j), sent to parent
-          ; /\ maybe the children have terminated?     
-          ) 
+          (b* ((val (erl-state->in (proc->s proc)))
+               ((unless (equal (erl-val-kind val) :integer)) nil)
+               (val (erl-val-integer->val val))
+               ((if (null children)) (equal val index))
+               (cpid (rightmost-child proc net))
+               (cproc (omap::lookup cpid net))
+               (cbind (erl-state->bind (proc->s cproc)))
+               (cindex (omap::lookup 'Index cbind)))
+              (and
+                ; the value must be the sum of indices of this branch.
+                (equal val (sum-range index cindex))
+                ; message sent must be well formed, if any
+                (sent-message-wf pid (proc->outbox proc) parent net)
+                ; all messages have been received already   
+                (null (proc->inbox-tried proc))
+                (null (proc->inbox-new proc))
+                ; ???: all children are terminated?
+                )))   
         (:blocked
-          ; /\ equal s->in :receive of next CPid
-          ; /\
-          ;    /\ s->bind Cpids correct regards to receive in s
-          ;    /\ s->LeftTotal contains f(i, (index (car CPid)))
-          ; /\ outbox is empty?
-          ; /\
-          ;   /\ inbox does not contain message from (car CPid).
-          ;   /\ all messages in inbox contain the correct values.
-          )
+          (b* (; if the node has no children, then it should not have blocked.
+               ((if (null children)) nil)
+              
+               ; during receive the latest value is wiped.
+               (val (erl-state->in (proc->s proc)))
+               ((unless (equal (erl-val-kind val) :none)) nil)
+
+               ; Ensure the existance of bindings created during the reduce call.
+               ((unless (omap::assoc 'ParentPid bind)) nil)
+               ((unless (omap::assoc 'CPids bind)) nil)
+               ((unless (omap::assoc 'ChildHd bind)) nil)
+               ((unless (omap::assoc 'ChildTl bind)) nil)
+               ((unless (omap::assoc 'LeftTotal bind)) nil)
+               
+               ; Parent never changes.
+               ((unless (equal parent (omap::lookup 'ParentPid bind))) nil)
+               
+               ; the childpids are a non-empty list
+               (cps (omap::lookup 'CPids bind))
+               ((unless (equal (erl-val-kind Cps) :cons)) nil)
+               (cps (erl-val-cons->lst cps))
+               ((unless cps) nil)
+               ; TODO: I might need a better representation for this:
+               ; The remaining children are a postfix of the original children.
+               ; sublist might be sufficient.
+               ((unless (prefixp (rev cps) (rev children))))
+               
+               ; ChildHead and ChildTail are bound correctly.
+               (chd (omap::lookup 'ChildHead bind))
+               ((unless (equal chd (car cps))) nil)
+               (ctl (omap::lookup 'ChildTail bind))
+               ((unless (equal (erl-val-kind ctl) :cons)) nil)
+               (ctl (erl-val-cons->lst ctl))
+               ((unless (equal ctl (cdr cps))) nil)
+
+               ; Acquire the index of the ChildHead
+               ; we should know from the preix that chd is a valid pid.
+               (chdproc (omap::lookup chd net))
+               (chdbind (erl-state->bind (proc->s chdproc)))
+               (cindex (omap::lookup 'Index chdbind))
+
+               ; LeftTotal
+               (lt (omap::lookup 'LeftTotal bind))
+               ((unless (equal lt (sum-range index (1- cindex)))))
+
+               ; The outbox must be empty, as the process will only send a
+               ; message when it is done computing the sum.
+               ((unless (null (proc->outbox proc))) nil)
+               ; ??? The parent, if any, must not have received the message yet.
+               ; However, this could be a property of the parent.
+
+               ; The world and module do not change
+               ((unless (equal (erl-state->world (proc->s proc)) (sum-reduce-w))) nil)
+               ((unless (equal (erl-state->module (proc->s proc)) 'local)) nil)
+
+               ; Inbox-new is empty, else the process would be unblocked
+               ((unless (null (proc->inbox-new proc))) nil)
+
+               ; Inbox-tried does not contain chd, otherwise the process would
+               ; have continued.
+               (inbox (proc->inbox-tried proc))
+               ((unless (received-messages-wf inbox cps net)) nil)
+               ((if (inbox-contains inbox chd)) nil)
+
+               ; ???: For messages not have yet received;
+               ; the sender is either
+               ; - not terminated
+               ; - or has the message in the outbox
+
+               ; Klst is correct
+               (klst (proc->klst proc))
+               (rbind
+                (omap::from-lists
+                  (list 'ChildPids 'Parent 'Index)
+                  (list (make-erl-val-cons :lst children)
+                        parent
+                        (make-erl-val-integer :val index))))
+               ((unless (reduce-receive-klst-p klst rbind)) t))
+             ; Check that there is no deadlock
+             (not (terminated? net))))
         (:receive
-          ; /\ equal s->in :receive of next CPid
-          ; /\
-          ;    /\ s->bind Cpids correct regards to receive in s
-          ;    /\ s->LeftTotal contains f(i, (index (car CPid)))
-          ; /\ outbox is empty?
-          ; /\ all messages in inbox contain the correct values.
-          ; /\ next message to receive is not in inbox tried?
-          ))))
+          (b* (; if the node has no children, then it should not try to receive.
+               ((if (null children)) nil)
+              
+               ; during receive the latest value is wiped.
+               (val (erl-state->in (proc->s proc)))
+               ((unless (equal (erl-val-kind val) :none)) nil)
+
+               ; Ensure the existance of bindings created during the reduce call.
+               ((unless (omap::assoc 'ParentPid bind)) nil)
+               ((unless (omap::assoc 'CPids bind)) nil)
+               ((unless (omap::assoc 'ChildHd bind)) nil)
+               ((unless (omap::assoc 'ChildTl bind)) nil)
+               ((unless (omap::assoc 'LeftTotal bind)) nil)
+               
+               ; Parent never changes.
+               ((unless (equal parent (omap::lookup 'ParentPid bind))) nil)
+               
+               ; the childpids are a non-empty list
+               (cps (omap::lookup 'CPids bind))
+               ((unless (equal (erl-val-kind Cps) :cons)) nil)
+               (cps (erl-val-cons->lst cps))
+               ((unless cps) nil)
+               ; TODO: I might need a better representation for this:
+               ; The remaining children are a postfix of the original children.
+               ; sublist might be sufficient.
+               ((unless (prefixp (rev cps) (rev children))))
+               
+               ; ChildHead and ChildTail are bound correctly.
+               (chd (omap::lookup 'ChildHead bind))
+               ((unless (equal chd (car cps))) nil)
+               (ctl (omap::lookup 'ChildTail bind))
+               ((unless (equal (erl-val-kind ctl) :cons)) nil)
+               (ctl (erl-val-cons->lst ctl))
+               ((unless (equal ctl (cdr cps))) nil)
+
+               ; Acquire the index of the ChildHead
+               ; we should know from the preix that chd is a valid pid.
+               (chdproc (omap::lookup chd net))
+               (chdbind (erl-state->bind (proc->s chdproc)))
+               (cindex (omap::lookup 'Index chdbind))
+
+               ; LeftTotal
+               (lt (omap::lookup 'LeftTotal bind))
+               ((unless (equal lt (sum-range index (1- cindex)))))
+
+               ; The outbox must be empty, as the process will only send a
+               ; message when it is done computing the sum.
+               ((unless (null (proc->outbox proc))) nil)
+               ; ??? The parent, if any, must not have received the message yet.
+               ; However, this could be a property of the parent.
+
+               ; The world and module do not change
+               ((unless (equal (erl-state->world (proc->s proc)) (sum-reduce-w))) nil)
+               ((unless (equal (erl-state->module (proc->s proc)) 'local)) nil)
+
+               ; Inbox-tried is empty, because the process has not started
+               ;  attempting to receive yet.
+               ((unless (null (proc->inbox-tried proc))) nil)
+
+               ; Inbox-new contains valid messages.
+               (inbox (proc->inbox-tried proc))
+               ((unless (received-messages-wf inbox cps net)) nil)
+               
+               ;???: For messages not have yet received;
+               ; the sender is either
+               ; - not terminated
+               ; - or has the message in the outbox
+
+               ; Klst is correct
+               (klst (proc->klst proc))
+               (rbind
+                (omap::from-lists
+                  (list 'ChildPids 'Parent 'Index)
+                  (list (make-erl-val-cons :lst children)
+                        parent
+                        (make-erl-val-integer :val index))))
+               ((unless (reduce-receive-klst-p klst rbind)) t))
+             ; Check that there is no deadlock
+             (not (terminated? net))))))
+  ///
+    (defcong pid-equiv equal (inv pid net) 1)
+    (defcong network-equiv equal (inv pid net) 2))
 
 
 ; The invariant for reduce
